Add within_size_class precondition for getsize + nlarith proofs

src/Main.fst
@@ -1315,24 +1315,95 @@ let slab_free' (i:US.t{US.v i < US.v nb_size_classes * US.v nb_arenas}) (ptr: ar
 
 #restart-solver
 
-// within_bounds model is awkward, am I just tired?
+
+/// Precondition of free, capturing that a client must return an array corresponding to the
+/// entire memory provided by the allocator:
+/// If a pointer is within a size class and aligned with
+/// the slots, then its length corresponds to the slot size
+let within_size_class_i (ptr:A.array U8.t) (sc: size_class_struct) : prop = (
+  // If ptr is within the size class sc
+  same_base_array sc.slab_region ptr /\
+  A.offset (A.ptr_of ptr) - A.offset (ptr_of (G.reveal sc.slab_region)) >= 0 /\
+  A.offset (A.ptr_of ptr) - A.offset (ptr_of (G.reveal sc.slab_region)) < US.v slab_size /\
+  // and it is aligned on the slots
+  (A.offset (A.ptr_of ptr) - A.offset (ptr_of (G.reveal sc.slab_region))) % U32.v sc.size = 0) ==>
+    // then its length is the length of a slot
+    A.length ptr == U32.v sc.size
+
+#push-options "--z3rlimit 100"
+/// Elimination lemma for `within_size_class_i`, triggering F* to prove the precondition
+/// of the implication
+let elim_within_size_class_i (ptr:A.array U8.t) (i:nat{i < Seq.length sc_all.g_size_classes}) (size:sc)
+  : Lemma (requires (let sc : size_class = G.reveal (Seq.index sc_all.g_size_classes i) in
+  size == sc.data.size /\
+  within_size_class_i ptr sc.data /\
+  same_base_array sc.data.slab_region ptr /\
+  A.offset (A.ptr_of ptr) - A.offset (ptr_of (G.reveal sc.data.slab_region)) >= 0 /\
+  A.offset (A.ptr_of ptr) - A.offset (ptr_of (G.reveal sc.data.slab_region)) < US.v slab_size /\
+  (A.offset (A.ptr_of ptr) - A.offset (ptr_of (G.reveal sc_all.slab_region))) % U32.v size = 0))
+    (ensures A.length ptr == U32.v size)
+  = let sc : size_class = G.reveal (Seq.index sc_all.g_size_classes i) in
+    let off_ptr = A.offset (A.ptr_of ptr) in
+    let off1 = A.offset (A.ptr_of (G.reveal sc_all.slab_region)) in
+    let off2 = A.offset (A.ptr_of (G.reveal sc.data.slab_region)) in
+    assert (off2 - off1 = i * US.v slab_size);
+    let div = U32.v page_size / U32.v size in
+    assert (US.v slab_size == (US.v metadata_max * div) * U32.v size);
+    let n = U32.v size in
+    Math.Lemmas.div_exact_r (U32.v page_size) n;
+    assert (n * div == U32.v page_size);
+    calc (==) {
+      off1 % n;
+      (==) { Math.Lemmas.modulo_modulo_lemma off1 n div }
+      (off1 % U32.v page_size) % n;
+      (==) { Math.Lemmas.lemma_mod_plus off1 (US.v metadata_max * i) (U32.v page_size) }
+      (off2 % U32.v page_size) % n;
+      (==) { Math.Lemmas.modulo_modulo_lemma off2 n div }
+      off2 % n;
+    };
+    calc (==) {
+      (off_ptr - off1) % n;
+      (==) { Math.Lemmas.lemma_mod_sub_distr off_ptr off1 n }
+      (off_ptr - off1 % n) % n;
+      (==) { }
+      (off_ptr - off2 % n) % n;
+      (==) { Math.Lemmas.lemma_mod_sub_distr off_ptr off2 n }
+      (off_ptr - off2) % n;
+    }
+#pop-options
+
+let within_size_classes_pred (ptr:A.array U8.t) : prop =
+  forall (i:nat{i < Seq.length sc_all.g_size_classes}).
+    within_size_class_i ptr (Seq.index (G.reveal sc_all.g_size_classes) i).data
+
+/// Auxiliary lemma to reason about the non-linear arithmetic for pointer division/modulo
+/// in a smaller context
+let lemma_nlarith_aux (n:US.t) (size:sc) : Lemma
+  (US.v (US.rem (US.rem n slab_size) (US.uint32_to_sizet size)) == US.v n % U32.v size)
+  = assert (US.v slab_size == US.v metadata_max * U32.v page_size);
+    assert (U32.v page_size % U32.v size == 0);
+    let div = U32.v page_size / U32.v size in
+    assert (US.v slab_size == (US.v metadata_max * div) * U32.v size);
+    calc (==) {
+      US.v (US.rem (US.rem n slab_size) (US.uint32_to_sizet size));
+      (==) { }
+      US.v (US.rem n slab_size) % (U32.v size);
+      (==) { }
+      (US.v n % US.v slab_size) % U32.v size;
+      (==) { Math.Lemmas.modulo_modulo_lemma (US.v n) (U32.v size) (US.v metadata_max * div) }
+      US.v n % U32.v size;
+    }
+
+#restart-solver
+#push-options "--z3rlimit 200"
+
 let slab_getsize (ptr: array U8.t)
   : Steel US.t
   (A.varray ptr `star` A.varray (A.split_l sc_all.slab_region 0sz))
   (fun _ ->
    A.varray ptr `star` A.varray (A.split_l sc_all.slab_region 0sz))
   (requires fun _ ->
-    //let x = offset (ptr_of ptr) - offset (ptr_of sc_all.slab_region) in
-    //((x >= 0 /\ x < US.v slab_region_size) ==> (
-    //  (let y = x / US.v slab_size in
-    //  0 <= y /\ y < Seq.length sc_all.g_sizes /\
-    //  (let sc = Seq.index sc_all.g_sizes y in
-    //    (x % US.v slab_size) % (U32.v sc) == 0
-    //    ==>
-    //    A.length ptr == U32.v sc
-    //  ))
-    //))
-    ///\
+    within_size_classes_pred ptr /\
     SAA.within_bounds
       (A.split_l (G.reveal sc_all.slab_region) 0sz)
       ptr
@@ -1369,9 +1440,10 @@ let slab_getsize (ptr: array U8.t)
   let size = ROArray.index sc_all.ro_sizes index in
   // some refactor needed wrt SlotsFree
   if US.rem rem (US.uint32_to_sizet size) = 0sz then (
-    // TODO: remove assume
-    // thanks to the ugly precondition
-    assume (A.length ptr == U32.v size);
+    (**) let sc = G.hide (Seq.index (G.reveal sc_all.g_size_classes) (US.v index)) in
+    lemma_nlarith_aux diff_sz size;
+    (**) elim_within_size_class_i ptr (US.v index) size;
+    (**) assert (A.length ptr == U32.v size);
     if enable_slab_canaries_malloc then
       return (US.uint32_to_sizet (size `U32.sub` 2ul))
     else
